Revert commits r2435 and r2436 (coarser RTLtyping / finer Lineartyping): the new Lineartyping can't keep track of single floats that were spilled.
git-svn-id: https://yquem.inria.fr/compcert/svn/compcert/trunk@2438 fca1b0fc-160b-0410-b1d3-a4f43f01ea2e

backend/Lineartyping.v
@@ -10,26 +10,20 @@
 (*                                                                     *)
 (* *********************************************************************)
 
-(** Type-checking Linear code. *)
+(** Typing rules for Linear. *)
 
-Require Import FSets.
-Require FSetAVL.
 Require Import Coqlib.
-Require Import Ordered.
-Require Import Maps.
-Require Import Iteration.
 Require Import AST.
 Require Import Integers.
 Require Import Values.
 Require Import Events.
 Require Import Op.
-Require Import Machregs.
 Require Import Locations.
 Require Import Conventions.
 Require Import LTL.
 Require Import Linear.
 
-(** The typechecker for Linear enforce several properties useful for
+(** The typing rules for Linear enforce several properties useful for
   the proof of the [Stacking] pass:
 - for each instruction, the type of the result register or slot
   agrees with the type of values produced by the instruction;
@@ -37,119 +31,12 @@ Require Import Linear.
   accessed through [Lgetstack] and [Lsetstack] Linear instructions.
 *)
 
-(** * Tracking the flow of single-precision floats *)
-
-(** At each program point, we infer a set of machine registers
-  that are guaranteed to contain single-precision floats.
-  The inference is a simple forward dataflow analysis, iterating on the 
-  list of instructions until a fixpoint is reached.  The result of
-  the analysis is a map from labels to sets of machine registers
-  containing single-precision floats.  *)
-
-Module OrderedMreg := OrderedIndexed(IndexedMreg).
-Module Regset := FSetAVL.Make(OrderedMreg).
-
-Definition setreg (fs: Regset.t) (r: mreg) (t: typ) :=
-  if typ_eq t Tsingle then Regset.add r fs else Regset.remove r fs.
-
-Fixpoint setregs (fs: Regset.t) (rl: list mreg) (tl: list typ) :=
-  match rl, tl with
-  | nil, nil => fs
-  | r1 :: rs, t1 :: ts => setregs (setreg fs r1 t1) rs ts
-  | _, _ => fs
-  end.
-
-Definition copyreg (fs: Regset.t) (rd rs: mreg) :=
-  if Regset.mem rs fs then Regset.add rd fs else Regset.remove rd fs.
-
-Definition allregs :=
-  List.fold_right Regset.add Regset.empty
-                  (float_caller_save_regs ++ float_callee_save_regs).
-
-Definition destroyed_at_call_regs :=
-  List.fold_right Regset.add Regset.empty destroyed_at_call.
-
-Definition callregs (fs: Regset.t) :=
-  Regset.diff fs destroyed_at_call_regs.
-
-Definition labelmap := PMap.t Regset.t.
-
-Definition update_label (lbl: label) (fs: Regset.t) (lm: labelmap) : Regset.t * labelmap * bool :=
-  let fs1 := PMap.get lbl lm in
-  if Regset.subset fs1 fs
-  then (fs1, lm, false)
-  else let fs2 := Regset.inter fs fs1 in (fs2, PMap.set lbl fs2 lm, true).
-
-Fixpoint update_labels (lbls: list label) (fs: Regset.t) (lm: labelmap): labelmap * bool :=
-  match lbls with
-  | nil => (lm, false)
-  | lbl1 :: lbls =>
-      let '(fs1, lm1, changed1) := update_label lbl1 fs lm in
-      let '(lm2, changed2) := update_labels lbls fs lm1 in
-      (lm2, changed1 || changed2)
-  end.
-
-Fixpoint ana_code (lm: labelmap) (ch: bool) (fs: Regset.t) (c: code) : labelmap * bool :=
-  match c with
-  | nil => (lm, ch)
-  | Lgetstack sl ofs ty rd :: c =>
-      ana_code lm ch (setreg fs rd ty) c
-  | Lsetstack rs sl ofs ty :: c =>
-      ana_code lm ch fs c
-  | Lop op args dst :: c =>
-      match is_move_operation op args with
-      | Some src => ana_code lm ch (copyreg fs dst src) c
-      | None     => ana_code lm ch (setreg fs dst (snd (type_of_operation op))) c
-      end
-  | Lload chunk addr args dst :: c =>
-      ana_code lm ch (setreg fs dst (type_of_chunk chunk)) c
-  | Lstore chunk addr args src :: c =>
-      ana_code lm ch fs c
-  | Lcall sg ros :: c =>
-      ana_code lm ch (callregs fs) c
-  | Ltailcall sg ros :: c =>
-      ana_code lm ch allregs c
-  | Lbuiltin ef args res :: c =>
-      ana_code lm ch (setregs fs res (proj_sig_res' (ef_sig ef))) c
-  | Lannot ef args :: c =>
-      ana_code lm ch fs c
-  | Llabel lbl :: c =>
-      let '(fs1, lm1, ch1) := update_label lbl fs lm in
-      ana_code lm1 (ch || ch1) fs1 c
-  | Lgoto lbl :: c =>
-      let '(fs1, lm1, ch1) := update_label lbl fs lm in
-      ana_code lm1 (ch || ch1) allregs c
-  | Lcond cond args lbl :: c =>
-      let '(fs1, lm1, ch1) := update_label lbl fs lm in
-      ana_code lm1 (ch || ch1) fs c
-  | Ljumptable r lbls :: c =>
-      let '(lm1, ch1) := update_labels lbls fs lm in
-      ana_code lm1 (ch || ch1) allregs c
-  | Lreturn :: c =>
-      ana_code lm ch allregs c
-  end.
-
-Definition ana_iter (c: code) (lm: labelmap) : labelmap + labelmap :=
-  let '(lm1, ch) := ana_code lm false Regset.empty c in
-  if ch then inr _ lm1 else inl _ lm.
-
-Definition ana_function (f: function): option (PMap.t Regset.t) :=
-  PrimIter.iterate _ _ (ana_iter f.(fn_code)) (PMap.init allregs).
-
-(** * The type-checker *)
-
-(** The typing rules are presented as boolean-valued functions so that we
+(** The rules are presented as boolean-valued functions so that we
   get an executable type-checker for free. *)
 
 Section WT_INSTR.
 
 Variable funct: function.
-
-Variable lm: labelmap.
-
-Definition reg_type (fs: Regset.t) (r: mreg) :=
-  let ty := mreg_type r in
-  if typ_eq ty Tfloat && Regset.mem r fs then Tsingle else ty.
 
 Definition slot_valid (sl: slot) (ofs: Z) (ty: typ): bool :=
   match sl with
@@ -176,579 +63,116 @@ Definition loc_valid (l: loc) : bool :=
   | S _ _ _ => false
   end.
 
-Fixpoint wt_code (fs: Regset.t) (c: code) : bool :=
-  match c with
-  | nil => true
-  | Lgetstack sl ofs ty rd :: c =>
-      subtype ty (mreg_type rd) && slot_valid sl ofs ty &&
-      wt_code (setreg fs rd ty) c
-  | Lsetstack rs sl ofs ty :: c =>
-      subtype (reg_type fs rs) ty &&
-      slot_valid sl ofs ty && slot_writable sl &&
-      wt_code fs c
-  | Lop op args dst :: c =>
+Definition wt_instr (i: instruction) : bool :=
+  match i with
+  | Lgetstack sl ofs ty r =>
+      subtype ty (mreg_type r) && slot_valid sl ofs ty
+  | Lsetstack r sl ofs ty =>
+      slot_valid sl ofs ty && slot_writable sl
+  | Lop op args res =>
       match is_move_operation op args with
-      | Some src =>
-          typ_eq (mreg_type src) (mreg_type dst) &&
-          wt_code (copyreg fs dst src) c
-      | None =>
-          let (ty_args, ty_res) := type_of_operation op in
-          subtype ty_res (mreg_type dst) &&
-          wt_code (setreg fs dst ty_res) c
+      | Some arg =>
+          subtype (mreg_type arg) (mreg_type res)
+      | None => 
+          let (targs, tres) := type_of_operation op in
+          subtype tres (mreg_type res)
       end
-  | Lload chunk addr args dst :: c =>
-      subtype (type_of_chunk chunk) (mreg_type dst) &&
-      wt_code (setreg fs dst (type_of_chunk chunk)) c
-  | Lstore chunk addr args src :: c =>
-      wt_code fs c
-  | Lcall sg ros :: c =>
-      wt_code (callregs fs) c
-  | Ltailcall sg ros :: c =>
-      zeq (size_arguments sg) 0 &&
-      wt_code allregs c
-  | Lbuiltin ef args res :: c =>
-      let ty_res := proj_sig_res' (ef_sig ef) in
-      subtype_list ty_res (map mreg_type res) &&
-      wt_code (setregs fs res ty_res) c
-  | Lannot ef args :: c =>
-      forallb loc_valid args &&
-      wt_code fs c
-  | Llabel lbl :: c =>
-      let fs1 := PMap.get lbl lm in
-      Regset.subset fs1 fs && wt_code fs1 c
-  | Lgoto lbl :: c =>
-      let fs1 := PMap.get lbl lm in
-      Regset.subset fs1 fs && wt_code allregs c
-  | Lcond cond args lbl :: c =>
-      let fs1 := PMap.get lbl lm in
-      Regset.subset fs1 fs && wt_code fs c
-  | Ljumptable r lbls :: c =>
-      forallb (fun lbl => Regset.subset (PMap.get lbl lm) fs) lbls &&
-      wt_code allregs c
-  | Lreturn :: c =>
-      wt_code allregs c
+  | Lload chunk addr args dst =>
+      subtype (type_of_chunk chunk) (mreg_type dst)
+  | Ltailcall sg ros =>
+      zeq (size_arguments sg) 0
+  | Lbuiltin ef args res =>
+      subtype_list (proj_sig_res' (ef_sig ef)) (map mreg_type res) 
+  | Lannot ef args =>
+      forallb loc_valid args
+  | _ =>
+      true
   end.
-
-Remark wt_code_cons:
-  forall fs i c,
-  wt_code fs (i :: c) = true -> exists fs', wt_code fs' c = true.
-Proof.
-  simpl; intros. destruct i; InvBooleans; try (econstructor; eassumption).
-  destruct (is_move_operation o l).
-  InvBooleans; econstructor; eassumption.
-  destruct (type_of_operation o). InvBooleans; econstructor; eassumption.
-Qed.
-
-Lemma wt_find_label:
-  forall lbl c' c fs,
-  find_label lbl c = Some c' ->
-  wt_code fs c = true ->
-  wt_code (PMap.get lbl lm) c' = true.
-Proof.
-  induction c; intros.
-- discriminate.
-- simpl in H. specialize (is_label_correct lbl a). destruct (is_label lbl a); intros IL.
-  + subst a. simpl in H0. inv H. InvBooleans. auto. 
-  + destruct (wt_code_cons _ _ _ H0) as [fs' WT]. eauto. 
-Qed.
 
 End WT_INSTR.
 
-Definition wt_funcode (f: function) (lm: labelmap) : bool :=
-  wt_code f lm Regset.empty f.(fn_code).
+Definition wt_code (f: function) (c: code) : bool :=
+  forallb (wt_instr f) c.
 
 Definition wt_function (f: function) : bool :=
-  match ana_function f with
-  | None => false
-  | Some lm => wt_funcode f lm
-  end.
+  wt_code f f.(fn_code).
 
-(** * Soundness of the type system *)
+(** Typing the run-time state.  These definitions are used in [Stackingproof]. *)
 
 Require Import Values.
-Require Import Globalenvs.
-Require Import Memory.
 
-Module RSF := FSetFacts.Facts(Regset).
-
-(** ** Typing the run-time state *)
-
-Definition loc_type (fs: Regset.t) (l: loc): typ :=
-  match l with
-  | R r => reg_type fs r
-  | S sl ofs ty => ty
-  end.
-
-Definition wt_locset (fs: Regset.t) (ls: locset) : Prop :=
-  forall l, Val.has_type (ls l) (loc_type fs l).
-
-Remark subtype_refl:
-  forall ty, subtype ty ty = true.
-Proof.
-  destruct ty; reflexivity.
-Qed.
-
-Remark reg_type_sub:
-  forall fs r, subtype (reg_type fs r) (mreg_type r) = true.
-Proof.
-  intros. unfold reg_type. destruct (typ_eq (mreg_type r) Tfloat); simpl.
-  rewrite e. destruct (Regset.mem r fs); auto. 
-  apply subtype_refl.
-Qed.
-
-Lemma wt_mreg:
-  forall fs ls r, wt_locset fs ls -> Val.has_type (ls (R r)) (mreg_type r).
-Proof.
-  intros. eapply Val.has_subtype. apply reg_type_sub with (fs := fs). apply H.
-Qed.
-
-Lemma wt_locset_empty:
-  forall ls,
-  (forall l, Val.has_type (ls l) (Loc.type l)) -> 
-  wt_locset Regset.empty ls.
-Proof.
-  intros; red; intros. destruct l; simpl.
-- unfold reg_type. change (Regset.mem r Regset.empty) with false. 
-  rewrite andb_false_r. apply H. 
-- apply H.
-Qed.
-
-Remark reg_type_mon:
-  forall fs1 fs2 r, Regset.Subset fs2 fs1 -> subtype (reg_type fs1 r) (reg_type fs2 r) = true.
-Proof.
-  intros. unfold reg_type. destruct (typ_eq (mreg_type r) Tfloat); simpl.
-  rewrite e. destruct (Regset.mem r fs2) eqn:E. 
-  rewrite Regset.mem_1. auto. apply H. apply Regset.mem_2; auto. 
-  destruct (Regset.mem r fs1); auto. 
-  apply subtype_refl.
-Qed.
-
-Lemma wt_locset_mon:
-  forall fs1 fs2 ls,
-  Regset.Subset fs2 fs1 -> wt_locset fs1 ls -> wt_locset fs2 ls.
-Proof.
-  intros; red; intros. apply Val.has_subtype with (loc_type fs1 l); auto. 
-  unfold loc_type. destruct l. apply reg_type_mon; auto. apply subtype_refl.
-Qed.
+Definition wt_locset (ls: locset) : Prop :=
+  forall l, Val.has_type (ls l) (Loc.type l).
 
 Lemma wt_setreg:
-  forall fs ls r v ty,
-  Val.has_type v ty -> subtype ty (mreg_type r) = true -> wt_locset fs ls ->
-  wt_locset (setreg fs r ty) (Locmap.set (R r) v ls).
+  forall ls r v,
+  Val.has_type v (mreg_type r) -> wt_locset ls -> wt_locset (Locmap.set (R r) v ls).
 Proof.
   intros; red; intros.
-  unfold Locmap.set. destruct (Loc.eq (R r) l).
-- subst l. simpl. unfold reg_type, setreg.
-  destruct (typ_eq (mreg_type r) Tfloat &&
-      Regset.mem r
-        (if typ_eq ty Tsingle then Regset.add r fs else Regset.remove r fs)) eqn:E.
-+ InvBooleans. destruct (typ_eq ty Tsingle).
-  congruence.
-  rewrite RSF.remove_b in H3. unfold RSF.eqb in H3. rewrite dec_eq_true in H3. 
-  simpl in H3. rewrite andb_false_r in H3. discriminate.
-+ eapply Val.has_subtype; eauto.
-- destruct (Loc.diff_dec (R r) l).
-+ replace (loc_type (setreg fs r ty) l) with (loc_type fs l).
-  apply H1. 
-  unfold loc_type, setreg. destruct l; auto. destruct (typ_eq ty Tsingle).
-  unfold reg_type. rewrite RSF.add_neq_b. auto. congruence. 
-  unfold reg_type. rewrite RSF.remove_neq_b. auto. congruence.
-+ red; auto. 
-Qed.
-
-Lemma wt_copyreg:
-  forall fs ls src dst v,
-  mreg_type src = mreg_type dst ->
-  wt_locset fs ls ->
-  Val.has_type v (reg_type fs src) ->
-  wt_locset (copyreg fs dst src) (Locmap.set (R dst) v ls).
-Proof.
-  intros; red; intros.
-  unfold Locmap.set. destruct (Loc.eq (R dst) l). 
-- subst l. simpl. unfold reg_type, copyreg.
-  unfold reg_type in H1. rewrite H in H1. 
-  destruct (Regset.mem src fs) eqn:SRC. 
-  rewrite RSF.add_b. unfold RSF.eqb. rewrite dec_eq_true. simpl. auto.
-  rewrite RSF.remove_b. unfold RSF.eqb. rewrite dec_eq_true. simpl. rewrite ! andb_false_r. 
-  rewrite andb_false_r in H1. auto.
-- destruct (Loc.diff_dec (R dst) l). 
-+ replace (loc_type (copyreg fs dst src) l) with (loc_type fs l).
-  apply H0.
-  unfold loc_type, copyreg. destruct l; auto. destruct (Regset.mem src fs). 
-  unfold reg_type. rewrite RSF.add_neq_b. auto. congruence. 
-  unfold reg_type. rewrite RSF.remove_neq_b. auto. congruence.
-+ red; auto.
+  unfold Locmap.set. 
+  destruct (Loc.eq (R r) l).
+  subst l; auto.
+  destruct (Loc.diff_dec (R r) l). auto. red. auto.
 Qed.
 
 Lemma wt_setstack:
-  forall fs ls sl ofs ty v,
-  Val.has_type v ty -> wt_locset fs ls ->
-  wt_locset fs (Locmap.set (S sl ofs ty) v ls).
+  forall ls sl ofs ty v,
+  wt_locset ls -> wt_locset (Locmap.set (S sl ofs ty) v ls).
 Proof.
   intros; red; intros.
   unfold Locmap.set. 
   destruct (Loc.eq (S sl ofs ty) l).
-  subst l. simpl. auto. 
+  subst l. simpl. 
+  generalize (Val.load_result_type (chunk_of_type ty) v). 
+  replace (type_of_chunk (chunk_of_type ty)) with ty. auto.
+  destruct ty; reflexivity.
   destruct (Loc.diff_dec (S sl ofs ty) l). auto. red. auto.
 Qed.
 
-Lemma wt_undef:
-  forall fs ls l, wt_locset fs ls -> wt_locset fs (Locmap.set l Vundef ls).
-Proof.
-  intros; red; intros. unfold Locmap.set. 
-  destruct (Loc.eq l l0). red; auto. 
-  destruct (Loc.diff_dec l l0); auto. red; auto.
-Qed.
-
 Lemma wt_undef_regs:
-  forall fs rs ls, wt_locset fs ls -> wt_locset fs (undef_regs rs ls).
+  forall rs ls, wt_locset ls -> wt_locset (undef_regs rs ls).
 Proof.
-  induction rs; simpl; intros. auto. apply wt_undef; auto. 
+  induction rs; simpl; intros. auto. apply wt_setreg; auto. red; auto.
 Qed.
 
 Lemma wt_call_regs:
-  forall fs ls, wt_locset fs ls -> wt_locset Regset.empty (call_regs ls).
+  forall ls, wt_locset ls -> wt_locset (call_regs ls).
 Proof.
-  intros; red; intros. unfold call_regs. destruct l.
-  eapply Val.has_subtype; eauto. unfold loc_type. apply reg_type_mon. 
-  red; intros. eelim Regset.empty_1; eauto. 
+  intros; red; intros. unfold call_regs. destruct l. auto.
   destruct sl.
   red; auto.
-  change (loc_type Regset.empty (S Incoming pos ty))
-    with (loc_type fs (S Outgoing pos ty)). auto.
+  change (Loc.type (S Incoming pos ty)) with (Loc.type (S Outgoing pos ty)). auto.
   red; auto.
-Qed.
-
-Remark set_from_list:
-  forall r l, Regset.In r (List.fold_right Regset.add Regset.empty l) <-> In r l.
-Proof.
-  induction l; simpl. 
-- rewrite RSF.empty_iff. tauto.
-- rewrite RSF.add_iff. rewrite IHl. tauto.
 Qed.
 
 Lemma wt_return_regs:
-  forall fs caller callee,
-  wt_locset fs caller -> wt_locset Regset.empty callee ->
-  wt_locset (callregs fs) (return_regs caller callee).
+  forall caller callee,
+  wt_locset caller -> wt_locset callee -> wt_locset (return_regs caller callee).
 Proof.
   intros; red; intros.
-  unfold return_regs. destruct l.
-- destruct (in_dec mreg_eq r destroyed_at_call). 
-+ unfold loc_type. replace (reg_type (callregs fs) r) with (mreg_type r).
-  eapply Val.has_subtype. eapply reg_type_sub. apply (H0 (R r)).
-  unfold reg_type, callregs. rewrite RSF.diff_b. 
-  rewrite (@Regset.mem_1 destroyed_at_call_regs).
-  rewrite ! andb_false_r. auto.
-  unfold destroyed_at_call_regs; apply set_from_list; auto.
-+ unfold loc_type, reg_type, callregs. rewrite RSF.diff_b. 
-  destruct (Regset.mem r destroyed_at_call_regs) eqn:E. 
-  elim n. apply set_from_list. apply Regset.mem_2; auto. 
-  rewrite andb_true_r. apply H. 
-- unfold loc_type. apply H. 
+  unfold return_regs. destruct l; auto.
+  destruct (in_dec mreg_eq r destroyed_at_call); auto.
 Qed.
 
 Lemma wt_init:
-  forall fs, wt_locset fs (Locmap.init Vundef).
+  wt_locset (Locmap.init Vundef).
 Proof.
   red; intros. unfold Locmap.init. red; auto.
 Qed.
 
-Lemma wt_setregs:
-  forall vl tyl rl fs rs,
-  Val.has_type_list vl tyl ->
-  subtype_list tyl (map mreg_type rl) = true ->
-  wt_locset fs rs ->
-  wt_locset (setregs fs rl tyl) (Locmap.setlist (map R rl) vl rs).
-Proof.
-  induction vl; simpl; intros.
-- destruct tyl; try contradiction. destruct rl; try discriminate. 
-  simpl. auto.
-- destruct tyl as [ | ty tyl]; try contradiction. destruct H.
-  destruct rl as [ | r rl]; simpl in H0; try discriminate. InvBooleans.
-  simpl. eapply IHvl; eauto. eapply wt_setreg; eauto. 
-Qed.
-
-Lemma wt_setregs_result:
-  forall sg fs v rl rs,
+Lemma wt_setlist_result:
+  forall sg v rs,
   Val.has_type v (proj_sig_res sg) ->
-  subtype_list (proj_sig_res' sg) (map mreg_type rl) = true ->
-  wt_locset fs rs ->
-  wt_locset (setregs fs rl (proj_sig_res' sg)) 
-            (Locmap.setlist (map R rl) (encode_long (sig_res sg) v) rs).
+  wt_locset rs ->
+  wt_locset (Locmap.setlist (map R (loc_result sg)) (encode_long (sig_res sg) v) rs).
 Proof.
-  intros. eapply wt_setregs; eauto. 
-  unfold proj_sig_res in H. unfold encode_long, proj_sig_res'. 
-  destruct (sig_res sg) as [[] | ]; simpl; intuition. 
-  destruct v; simpl; auto.
-  destruct v; simpl; auto.
-Qed.
-
-Remark in_setreg_other:
-  forall fs r ty r',
-  r' <> r -> (Regset.In r' (setreg fs r ty) <-> Regset.In r' fs).
-Proof.
-  intros. unfold setreg. destruct (typ_eq ty Tsingle). 
-  rewrite RSF.add_iff. intuition. 
-  rewrite RSF.remove_iff. intuition.
-Qed.
-
-Remark in_setregs_other:
-  forall r rl fs tyl,
-  ~In r rl -> (Regset.In r (setregs fs rl tyl) <-> Regset.In r fs).
-Proof.
-  induction rl; simpl; intros. 
-- destruct tyl; tauto.
-- destruct tyl. tauto. rewrite IHrl by tauto. apply in_setreg_other. intuition.
-Qed. 
-
-Remark callregs_setregs_result:
-  forall sg fs,
-  Regset.Subset (callregs fs) (setregs fs (loc_result sg) (proj_sig_res' sg)).
-Proof.
-  red; unfold callregs; intros. rewrite RSF.diff_iff in H. destruct H. 
-  apply in_setregs_other; auto. 
-  red; intros; elim H0. apply set_from_list. eapply loc_result_caller_save; eauto.
-Qed.
-
-Definition wt_fundef (fd: fundef) :=
-  match fd with
-  | Internal f => wt_function f = true
-  | External ef => True
-  end.
-
-Inductive wt_callstack: list stackframe -> Regset.t -> Prop :=
-  | wt_callstack_nil: forall fs, 
-      wt_callstack nil fs
-  | wt_callstack_cons: forall f sp rs c s fs lm fs0 fs1
-        (WTSTK: wt_callstack s fs0)
-        (WTF: wt_funcode f lm = true)
-        (WTC: wt_code f lm (callregs fs1) c = true)
-        (WTRS: wt_locset fs rs)
-        (INCL: Regset.Subset (callregs fs1) (callregs fs)),
-      wt_callstack (Stackframe f sp rs c :: s) fs.
-
-Lemma wt_parent_locset:
-  forall s fs, wt_callstack s fs -> wt_locset fs (parent_locset s).
-Proof.
-  induction 1; simpl.
-- apply wt_init.
-- auto.
-Qed.
-
-Lemma wt_callstack_change_fs:
-  forall s fs, wt_callstack s fs -> wt_callstack s (callregs fs).
-Proof.
-  induction 1.
-- constructor.
-- econstructor; eauto. 
-  apply wt_locset_mon with fs; auto. 
-  unfold callregs; red; intros. eapply Regset.diff_1; eauto.
-  red; intros. exploit INCL; eauto. unfold callregs. rewrite ! RSF.diff_iff. 
-  tauto.
-Qed.
-
-Inductive wt_state: state -> Prop :=
-  | wt_regular_state: forall s f sp c rs m lm fs fs0
-        (WTSTK: wt_callstack s fs0)
-        (WTF: wt_funcode f lm = true)
-        (WTC: wt_code f lm fs c = true)
-        (WTRS: wt_locset fs rs),
-      wt_state (State s f sp c rs m)
-  | wt_call_state: forall s fd rs m fs
-        (WTSTK: wt_callstack s fs)
-        (WTFD: wt_fundef fd)
-        (WTRS: wt_locset fs rs),
-      wt_state (Callstate s fd rs m)
-  | wt_return_state: forall s rs m fs
-        (WTSTK: wt_callstack s fs)
-        (WTRS: wt_locset (callregs fs) rs),
-      wt_state (Returnstate s rs m).
-
-(** ** Preservation of state typing by transitions *)
-
-Section SOUNDNESS.
-
-Variable prog: program.
-Let ge := Genv.globalenv prog.
-
-Hypothesis wt_prog:
-  forall i fd, In (i, Gfun fd) prog.(prog_defs) -> wt_fundef fd.
-
-Lemma wt_find_function:
-  forall ros rs f, find_function ge ros rs = Some f -> wt_fundef f.
-Proof.
-  intros. 
-  assert (X: exists i, In (i, Gfun f) prog.(prog_defs)).
-  {
-    destruct ros as [r | s]; simpl in H.
-    eapply Genv.find_funct_inversion; eauto. 
-    destruct (Genv.find_symbol ge s) as [b|]; try discriminate.
-    eapply Genv.find_funct_ptr_inversion; eauto.
-  }
-  destruct X as [i IN]. eapply wt_prog; eauto. 
-Qed.
-
-Theorem step_type_preservation:
-  forall S1 t S2, step ge S1 t S2 -> wt_state S1 -> wt_state S2.
-Proof.
-  induction 1; intros WTS; inv WTS.
-- (* getstack *)
-  simpl in WTC; InvBooleans. 
-  econstructor; eauto.
-  apply wt_setreg; auto. apply (WTRS (S sl ofs ty)). apply wt_undef_regs; auto.
-- (* setstack *)
-  simpl in WTC; InvBooleans. 
-  econstructor; eauto. 
-  apply wt_setstack; auto. eapply Val.has_subtype; eauto. apply WTRS. 
-  apply wt_undef_regs; auto.
-- (* op *)
-  simpl in WTC. destruct (is_move_operation op args) as [src | ] eqn:ISMOVE.
-  + (* move *)
-    InvBooleans. exploit is_move_operation_correct; eauto. intros [EQ1 EQ2]; subst. 
-    simpl in H. inv H.
-    econstructor; eauto. 
-    apply wt_copyreg. auto. apply wt_undef_regs; auto. apply WTRS. 
-  + (* other ops *) 
-    destruct (type_of_operation op) as [ty_args ty_res] eqn:TYOP. InvBooleans.
-    econstructor; eauto.
-    apply wt_setreg; auto. 
-    change ty_res with (snd (ty_args, ty_res)). rewrite <- TYOP. 
-    eapply type_of_operation_sound; eauto. 
-    red; intros; subst op. simpl in ISMOVE. 
-    destruct args; try discriminate. destruct args; discriminate. 
-    apply wt_undef_regs; auto.
-- (* load *)
-  simpl in WTC; InvBooleans. 
-  econstructor; eauto.
-  apply wt_setreg. 
-  destruct a; simpl in H0; try discriminate. eapply Mem.load_type; eauto.
-  auto. 
-  apply wt_undef_regs; auto.
-- (* store *)
-  simpl in WTC; InvBooleans. 
-  econstructor; eauto.
-  apply wt_undef_regs; auto.
-- (* call *)
-  simpl in WTC; InvBooleans.
-  econstructor; eauto. econstructor; eauto.
-  red; auto.
-  eapply wt_find_function; eauto.
-- (* tailcall *)
-  simpl in WTC; InvBooleans.
-  econstructor. apply wt_callstack_change_fs; eauto. 
-  eapply wt_find_function; eauto.
-  apply wt_return_regs. apply wt_parent_locset; auto. 
-  eapply wt_locset_mon; eauto. red; intros. eelim Regset.empty_1; eauto.
-- (* builtin *)
-  simpl in WTC; InvBooleans. inv H. 
-  econstructor; eauto.
-  apply wt_setregs_result; auto.
-  eapply external_call_well_typed; eauto.
-  apply wt_undef_regs; auto.
-- (* annot *)
-  simpl in WTC; InvBooleans.
-  econstructor; eauto. 
-- (* label *)
-  simpl in WTC; InvBooleans. 
-  econstructor; eauto.
-  eapply wt_locset_mon; eauto. apply Regset.subset_2; auto.
-- (* goto *)
-  simpl in WTC; InvBooleans. 
-  econstructor. eauto. eauto. 
-  eapply wt_find_label; eauto. 
-  eapply wt_locset_mon; eauto. apply Regset.subset_2; auto.
-- (* cond branch, taken *)
-  simpl in WTC; InvBooleans. 
-  econstructor. eauto. eauto. 
-  eapply wt_find_label; eauto. 
-  eapply wt_locset_mon. apply Regset.subset_2; eauto.
-  apply wt_undef_regs; auto.
-- (* cond branch, not taken *)
-  simpl in WTC; InvBooleans. 
-  econstructor. eauto. eauto. eauto. 
-  apply wt_undef_regs; auto.
-- (* jumptable *)
-  simpl in WTC; InvBooleans. 
-  econstructor. eauto. eauto.
-  eapply wt_find_label; eauto. 
-  apply wt_locset_mon with fs.
-  apply Regset.subset_2. rewrite List.forallb_forall in H2. apply H2. 
-  eapply list_nth_z_in; eauto.
-  apply wt_undef_regs; auto.
-- (* return *)
-  econstructor. eauto. 
-  apply wt_return_regs. 
-  apply wt_parent_locset; auto. 
-  apply wt_locset_mon with fs; auto. red; intros. eelim Regset.empty_1; eauto.
-- (* internal function *)
-  simpl in WTFD. unfold wt_function in WTFD. destruct (ana_function f) as [lm|]; try discriminate.
-  econstructor. eauto. eauto. eexact WTFD. 
-  apply wt_undef_regs. eapply wt_call_regs; eauto. 
-- (* external function *)
-  inv H0. 
-  econstructor. eauto. 
-  eapply wt_locset_mon. 2: eapply wt_setregs_result; eauto. 
-  apply callregs_setregs_result. 
-  eapply external_call_well_typed; eauto. 
-  unfold proj_sig_res', loc_result. destruct (sig_res (ef_sig ef) )as [[] | ]; auto.
-- (* return *)
-  inv WTSTK. econstructor; eauto. 
-  apply wt_locset_mon with (callregs fs); auto. 
-Qed.
-
-Theorem wt_initial_state:
-  forall S, initial_state prog S -> wt_state S.
-Proof.
-  induction 1. econstructor. 
-  apply wt_callstack_nil with (fs := Regset.empty).
-  unfold ge0 in H1. exploit Genv.find_funct_ptr_inversion; eauto.
-  intros [id IN]. eapply wt_prog; eauto. 
-  apply wt_init.
-Qed.
-
-End SOUNDNESS.
-
-(** Properties of well-typed states that are used in [Stackingproof]. *)
-
-Lemma wt_state_getstack:
-  forall s f sp sl ofs ty rd c rs m,
-  wt_state (State s f sp (Lgetstack sl ofs ty rd :: c) rs m) ->
-  slot_valid f sl ofs ty = true.
-Proof.
-  intros. inv H. simpl in WTC; InvBooleans. auto.
-Qed.
-
-Lemma wt_state_setstack:
-  forall s f sp sl ofs ty r c rs m,
-  wt_state (State s f sp (Lsetstack r sl ofs ty :: c) rs m) ->
-  Val.has_type (rs (R r)) ty /\ slot_valid f sl ofs ty = true /\ slot_writable sl = true.
-Proof.
-  intros. inv H. simpl in WTC; InvBooleans. intuition. 
-  eapply Val.has_subtype; eauto. apply WTRS. 
-Qed.
-
-Lemma wt_state_tailcall:
-  forall s f sp sg ros c rs m,
-  wt_state (State s f sp (Ltailcall sg ros :: c) rs m) ->
-  size_arguments sg = 0.
-Proof.
-  intros. inv H. simpl in WTC; InvBooleans. auto.
-Qed.
-
-Lemma wt_state_annot:
-  forall s f sp ef args c rs m,
-  wt_state (State s f sp (Lannot ef args :: c) rs m) ->
-  forallb (loc_valid f) args = true.
-Proof.
-  intros. inv H. simpl in WTC; InvBooleans. auto. 
-Qed.
-
-Lemma wt_callstate_wt_locset:
-  forall s f rs m,
-  wt_state (Callstate s f rs m) -> wt_locset Regset.empty rs.
-Proof.
-  intros. inv H. apply wt_locset_mon with fs; auto. 
-  red; intros; eelim Regset.empty_1; eauto.
+  unfold loc_result, encode_long, proj_sig_res; intros.
+  destruct (sig_res sg) as [[] | ]; simpl.
+- apply wt_setreg; auto.
+- apply wt_setreg; auto.
+- destruct v; simpl in H; try contradiction;
+  simpl; apply wt_setreg; auto; apply wt_setreg; auto.
+- apply wt_setreg; auto. apply Val.has_subtype with Tsingle; auto. 
+- apply wt_setreg; auto.
 Qed.
 
